\section*{Série 1 Página60  - 6}
    
    \subsection*{A)}
    $\int_{a}^{b}f(x)dx = \int_{0}^{1}(kx^2 - kx^3)dx = k [\int_{0}^{1}x^2dx - \int_{0}^{1}x^3dx] = k \bigg[\frac{x^3}{3}\Big|^1_0 - \frac{x^4}{4}\Big|^1_0\bigg] = k [(\frac{1^3}{3} - \frac{0^3}{3}) - (\frac{1^4}{4} - \frac{0^4}{4})] = k \times \frac{1}{12}\\
    \int_{0}^{1}f(x)dx = 1 \rightarrow k \times \frac{1}{12} = 1 \rightarrow k = 12$
    
    \subsection*{B)}
    $\int_{-\infty}^{+\infty}xf(x)dx = \int_{-\infty}^{+\infty}x[12(x^2 - x^3)]dx = \int_{0}^{1}12(x^3 - x^4)dx = 12\int_{0}^{1}x^3dx - \int_{0}^{1}x^4dx = \\
    12 \bigg[\frac{x^4}{4}\Big|^1_0 - \frac{x^5}{5}\Big|^1_0\bigg] = 12 [\frac{1}{4} - \frac{1}{5}] = \frac{12}{20} = \frac{3}{5}$
    
    
    \subsection*{C)}
    $\int_{0}^{md}12(x^2 - x^3)dx = 12 \bigg[\int_{0}^{md}x^2dx - \int_{0}^{md}x^3dx = 12\bigg[\frac{x^3}{3}\Big|^{md}_0 - \frac{x^4}{4}\Big|^{md}_0\bigg] = 4md^3 - 3md^4\\
    4md^3 - 3md^4 = 0,5$ 
    
